theories/Term.v
@@ -21,18 +21,220 @@ Implicit Type N: normal.
 Implicit Types x y: var.
 Implicit Type ρ: subst.
 
-Function typecheck Γ v t: bool :=
-  match v, t with
-  | v_tt, t_unit => true
-  | v_fanout v0 v1, t1 * t2 =>
-      typecheck Γ v0 t1 && typecheck Γ v1 t2
-  | v_neu v, _ =>
-      if typeinfer Γ v is Some t'
-      then if eq_type t t' then true else false
-      else false
-  | _, _ => false
-  end %bool
-with typeinfer Γ V :=
+Function η t V :=
+  match t with
+  | t_var _ => v_neu V
+  | t_unit => v_tt
+  | t1 * t2 =>
+      v_fanout (η t1 (V_fst V))  (η t2 (V_snd V))
+  end.
+
+Theorem η_preserve {t}:
+  ∀ {Γ V},
+  JV Γ V t →
+  Γ ⊢ η t V in t.
+Proof.
+  induction t.
+  all: cbn.
+  all: intros ? ? q.
+  - intros.
+    constructor.
+    auto.
+  - constructor.
+  - constructor.
+    + eapply IHt1.
+      econstructor.
+      eauto.
+    + eapply IHt2.
+      econstructor.
+      eauto.
+Qed.
+
+Function hsubst_expr v' x V :=
+  match V with
+  | V_var y => if eq_var x y then Some v' else None
+  | V_fst V =>
+      do v_fanout v1 _ ← hsubst_expr v' x V ;
+      Some v1
+  | V_snd V =>
+      do v_fanout _ v2 ← hsubst_expr v' x V ;
+      Some v2
+  end.
+
+Function hsubst_term v' x v :=
+  match v with
+  | v_tt => Some v_tt
+  | v_fanout v1 v2 =>
+      do v1' ← hsubst_term v' x v1 ;
+      do v2' ← hsubst_term v' x v2 ;
+      Some (v_fanout v1' v2')
+  | v_neu V => hsubst_expr v' x V
+  end.
+
+Lemma hsubst_preserve_expr {v' x V}:
+  ∀ {Γ t},
+    Γ ⊢ v' in t →
+  ∀ {t'},
+    JV (cons (x, t) Γ) V t' →
+    ∀ {vout}, hsubst_expr v' x V = Some vout →
+    Γ ⊢ vout in t'.
+Proof.
+  functional induction (hsubst_expr v' x V).
+  all: intros ? ? q ? p ? r.
+  all: inversion p.
+  all: subst.
+  all: clear p.
+  - inversion H1.
+    all: subst.
+    2: contradiction.
+    inversion r.
+    subst.
+    auto.
+  - inversion H1.
+    all: subst.
+    1: contradiction.
+    inversion r.
+  - inversion r.
+    subst.
+    clear r.
+    assert (e0' := IHo _ _ q _ H1 _ e0).
+    inversion e0'.
+    subst.
+    auto.
+  - inversion r.
+  - inversion r.
+    subst.
+    clear r.
+    assert (e0' := IHo _ _ q _ H1 _ e0).
+    inversion e0'.
+    subst.
+    auto.
+  - inversion r.
+Qed.
+
+Lemma hsubst_preserve_term {v' x v}:
+  ∀ {Γ t},
+    Γ ⊢ v' in t →
+  ∀ {t'},
+    (x, t) :: Γ ⊢ v in t' →
+    ∀ {vout}, hsubst_term v' x v = Some vout →
+    Γ ⊢ vout in t'.
+Proof.
+  functional induction (hsubst_term v' x v).
+  all: intros ? ? q ? p ? r.
+  all: inversion p.
+  all: subst.
+  all: clear p.
+  - inversion r.
+    all: subst.
+    constructor.
+  - inversion r.
+    all: subst.
+    constructor.
+    all: eauto.
+  - inversion r.
+  - inversion r.
+  - eapply hsubst_preserve_expr.
+    all: eauto.
+Qed.
+
+Lemma map_expr {Γ Γ'}:
+  (∀ x t, mem x t Γ → mem x t Γ') →
+  ∀ {V t}, JV Γ V t → JV Γ' V t.
+Proof using.
+  intros ? ? ? p.
+  induction p.
+  all: econstructor.
+  all: eauto.
+Qed.
+
+Lemma map_term {Γ Γ'}:
+  (∀ x t, mem x t Γ → mem x t Γ') →
+  ∀ {v t}, Γ ⊢ v in t → Γ' ⊢ v in t.
+Proof.
+  intros ? ? ? p.
+  induction p.
+  all: econstructor.
+  all: eauto.
+  eapply map_expr.
+  all: eauto.
+Qed.
+
+Lemma hsubst_expr_total {V}:
+  ∀ {x t' t},
+    JV (cons (x, t) nil) V t' →
+  ∀ {v' t''},
+  (x, t'') :: nil ⊢ v' in t →
+  ∃ vout, hsubst_expr v' x V = Some vout.
+Proof.
+  induction V.
+  all: cbn.
+  all: intros ? ? ? q.
+  all: inversion q.
+  all: clear q.
+  all: subst.
+  all: intros ? ? p.
+  - inversion H1.
+    all: subst.
+    + destruct eq_var.
+      2: contradiction.
+      eexists.
+      eauto.
+    + destruct eq_var.
+      1: subst; contradiction.
+      inversion H6.
+  - destruct (IHV _ _ _ H1 _ _ p) as [? q1].
+    rewrite q1.
+    eassert (H1' := hsubst_preserve_expr p _ q1).
+    Unshelve.
+    3: {
+      eapply (map_expr Environment.shadow).
+      eapply H1.
+    }
+    destruct x0.
+    all: inversion H1'.
+    eexists.
+    eauto.
+  - destruct (IHV _ _ _ H1 _ _ p) as [? q1].
+    rewrite q1.
+    eassert (H1' := hsubst_preserve_expr p _ q1).
+    Unshelve.
+    3: {
+      eapply (map_expr Environment.shadow).
+      eapply H1.
+    }
+    destruct x0.
+    all: inversion H1'.
+    eexists.
+    eauto.
+Qed.
+
+Lemma hsubst_term_total {v}:
+  ∀ {x t' t},
+    (x, t) :: nil ⊢ v in t' →
+  ∀ {v' t''},
+  (x, t'') :: nil ⊢ v' in t →
+  ∃ vout, hsubst_term v' x v = Some vout.
+Proof.
+  induction v.
+  all: cbn.
+  all: intros ? ? ? q.
+  all: inversion q.
+  all: clear q.
+  all: subst.
+  all: intros ? ? p.
+  - eexists.
+    eauto.
+  - destruct (IHv1 _ _ _ H2 _ _ p) as [? q1].
+    destruct (IHv2 _ _ _ H4 _ _ p) as [? q2].
+    rewrite q1, q2.
+    eexists.
+    eauto.
+  - eapply hsubst_expr_total.
+    all: eauto.
+Qed.
+
+Function typeinfer Γ V :=
   match V with
   | V_var x => find x Γ
   | V_fst V =>
@@ -41,11 +243,103 @@ with typeinfer Γ V :=
   | V_snd V =>
       do _ * t1 ← typeinfer Γ V ;
       Some t1
-  | V_cut v t =>
-      if typecheck Γ v t
-      then Some t
-      else None
   end.
+
+Function typecheck Γ v t: bool :=
+  match v, t with
+  | v_tt, t_unit => true
+  | v_fanout v0 v1, t1 * t2 =>
+      typecheck Γ v0 t1 && typecheck Γ v1 t2
+  | v_neu v, t_var _ =>
+      if typeinfer Γ v is Some t'
+      then if eq_type t t' then true else false
+      else false
+  | _, _ => false
+  end %bool.
+
+Function elim x s (V: expr) :=
+  match V with
+  | V_var y => if eq_var x y then Some s else None
+  | V_fst V =>
+      do v_fanout a _ ← elim x s V ;
+      Some a
+  | V_snd V =>
+      do v_fanout _ a ← elim x s V ;
+      Some a
+  end.
+
+Function intro x s v :=
+  match v with
+  | v_tt => Some v_tt
+  | v_fanout v0 v1 =>
+      do v0' ← intro x s v0 ;
+      do v1' ← intro x s v1 ;
+      Some (v_fanout v0' v1')
+  | v_neu V => elim x s V
+  end.
+
+Lemma elim_sound {x s V}:
+  ∀ {v'}, elim x s V = Some v' →
+  hsubstV x s V v'.
+Proof.
+  functional induction (elim x s V).
+  all: try discriminate.
+  all: intros ? p.
+  all: inversion p.
+  all: subst.
+  - constructor.
+  - econstructor.
+    eauto.
+  - econstructor.
+    eauto.
+Qed.
+
+Lemma intro_sound {x s v}:
+  ∀ {v'}, intro x s v = Some v' →
+  hsubstv x s v v'.
+Proof.
+  functional induction (intro x s v).
+  all: try discriminate.
+  all: intros ? p.
+  all: inversion p.
+  all: subst.
+  - constructor.
+  - constructor.
+    all: auto.
+  - constructor.
+    apply elim_sound.
+    auto.
+Qed.
+
+Lemma elim_complete {x s V v'}:
+  hsubstV x s V v' →
+  elim x s V = Some v'.
+Proof.
+  intro p.
+  induction p.
+  all: cbn.
+  - destruct eq_var.
+    2: contradiction.
+    auto.
+  - rewrite IHp.
+    auto.
+  - rewrite IHp.
+    auto.
+Qed.
+
+Lemma intro_complete {x s v v'}:
+  hsubstv x s v v' →
+  intro x s v = Some v'.
+Proof.
+  intro p.
+  induction p.
+  all: cbn.
+  - auto.
+  - rewrite IHp1, IHp2.
+    auto.
+  - apply elim_complete.
+    auto.
+Qed.
 
 Function lookup x ρ: option normal :=
   if ρ is ((y, t) :: ρ')%list
@@ -55,62 +349,10 @@ Function lookup x ρ: option normal :=
     else lookup x ρ'
   else None.
 
-Function intro ρ v :=
-  match v with
-  | v_tt => Some N_tt
-  | v_fanout v0 v1 =>
-      do v0' ← intro ρ v0 ;
-      do v1' ← intro ρ v1 ;
-      Some (N_fanout v0' v1')
-  | v_neu V => elim ρ V
-  end
-with elim ρ (V: expr) :=
-  match V with
-  | V_var x => lookup x ρ
-  | V_fst V =>
-      do N_fanout a _ ← elim ρ V ;
-      Some a
-  | V_snd V =>
-      do N_fanout _ a ← elim ρ V ;
-      Some a
-  | V_cut v _ => intro ρ v
-  end.
 
-Theorem typecheck_sound:
-  ∀ {Γ v t}, Bool.Is_true (typecheck Γ v t) → Γ ⊢ v in t
-with typeinfer_sound:
-  ∀ {Γ V t}, typeinfer Γ V = Some t → JV Γ V t.
+Fixpoint typeinfer_sound {Γ V t}: typeinfer Γ V = Some t → JV Γ V t.
 Proof using .
-  - intros Γ v t p.
-    destruct v.
-    all: cbn.
-    + destruct t.
-      all: try contradiction.
-      constructor.
-    + destruct t.
-      all: try contradiction.
-      cbn in p.
-      destruct typecheck eqn:q1.
-      2: contradiction.
-      destruct typecheck eqn:q2 in p.
-      2: contradiction.
-      constructor.
-      * apply typecheck_sound.
-        rewrite q1.
-        apply I.
-      * apply typecheck_sound.
-        rewrite q2.
-        apply I.
-    + cbn in p.
-      constructor.
-      apply typeinfer_sound.
-      destruct typeinfer.
-      2: contradiction.
-      destruct eq_type.
-      2: contradiction.
-      subst.
-      auto.
-  - intros Γ V t p.
+  - intros p.
     destruct V.
     all: cbn.
     + cbn in p.
@@ -137,36 +379,46 @@ Proof using .
       econstructor.
       apply typeinfer_sound.
       eauto.
-    + cbn in p.
-      destruct typecheck eqn:q.
-      2: discriminate.
-      inversion p.
-      subst.
-      constructor.
-      apply typecheck_sound.
-      rewrite q.
-      apply I.
 Qed.
 
-Theorem typecheck_complete:
-  ∀ {Γ v t}, Γ ⊢ v in t → typecheck Γ v t = true
-with typeinfer_complete:
-  ∀ {Γ V t}, JV Γ V t → typeinfer Γ V = Some t.
+Fixpoint typecheck_sound {Γ v t}:
+  Bool.Is_true (typecheck Γ v t) → Γ ⊢ v in t.
+  - intros p.
+    destruct v.
+    all: cbn.
+    + destruct t.
+      all: try contradiction.
+      constructor.
+    + destruct t.
+      all: try contradiction.
+      cbn in p.
+      destruct typecheck eqn:q1.
+      2: contradiction.
+      destruct typecheck eqn:q2 in p.
+      2: contradiction.
+      constructor.
+      * apply typecheck_sound.
+        rewrite q1.
+        apply I.
+      * apply typecheck_sound.
+        rewrite q2.
+        apply I.
+    + cbn in p.
+      destruct t.
+      all: try contradiction.
+      destruct typeinfer eqn:q.
+      all: try contradiction.
+      destruct eq_type.
+      all: try contradiction.
+      subst.
+      constructor.
+      apply typeinfer_sound.
+      auto.
+Qed.
+
+Fixpoint typeinfer_complete {Γ V t} (p: JV Γ V t): typeinfer Γ V = Some t.
 Proof using .
-  - intros Γ ? ? p.
-    destruct p.
-    all: cbn in *.
-    all: auto.
-    all: try rewrite typecheck_complete.
-    all: try rewrite typecheck_complete.
-    all: auto.
-    rewrite (typeinfer_complete Γ V t).
-    2: auto.
-    destruct eq_type.
-    2: contradiction.
-    auto.
-  - intros Γ ? ? p.
-    destruct p.
+  - destruct p.
     all: cbn in *.
     + apply find_complete.
       auto.
@@ -174,10 +426,21 @@ Proof using .
       auto.
     + rewrite (typeinfer_complete Γ V _ p).
       auto.
-    + rewrite typecheck_complete.
-      all: auto.
 Qed.
 
+Fixpoint typecheck_complete {Γ v t} (p: Γ ⊢ v in t): typecheck Γ v t = true.
+Proof using .
+  destruct p.
+  all: cbn in *.
+  all: auto.
+  all: try rewrite typecheck_complete.
+  all: try rewrite typecheck_complete.
+  all: auto.
+  rewrite (typeinfer_complete H).
+  destruct eq_tyvar.
+  2: contradiction.
+  auto.
+Qed.
 
 Lemma lookup_sound {x ρ}:
   ∀ {N}, lookup x ρ = Some N → memp x N ρ.
@@ -204,396 +467,29 @@ Proof using .
     auto.
 Qed.
 
-Theorem intro_sound {ρ v N}: intro ρ v = Some N → ρ ⊢ v ⇓ N
-with elim_sound {ρ V N}: elim ρ V = Some N → bigV ρ V N.
-Proof using.
-  - intro p.
-    destruct v.
-    all: cbn in p.
-    + inversion p.
-      constructor.
-    + destruct intro eqn:q1.
-      2: discriminate.
-      destruct intro eqn:q2 in p.
-      2: discriminate.
-      inversion p.
-      constructor.
-      all: auto.
-    + constructor.
-      apply elim_sound.
-      auto.
-  - intro p.
-    destruct V.
-    all: cbn in p.
-    + constructor.
-      apply lookup_sound.
-      auto.
-    + destruct elim eqn:q1.
-      2: discriminate.
-      destruct n.
-      1: discriminate.
-      inversion p.
-      subst.
-      econstructor.
-      eauto.
-    + destruct elim eqn:q1.
-      2: discriminate.
-      destruct n.
-      1: discriminate.
-      inversion p.
-      subst.
-      econstructor.
-      eauto.
-    + constructor.
-      apply intro_sound.
-      auto.
-Qed.
+Definition oftype Γ t := { v | Bool.Is_true (typecheck Γ v t) }.
 
-Theorem intro_complete {ρ v N}: ρ ⊢ v ⇓ N → intro ρ v = Some N
-with elim_complete {ρ V N}: bigV ρ V N → elim ρ V = Some N.
-Proof using.
-  - intros p.
-    destruct p.
-    all: cbn.
-    + auto.
-    + repeat erewrite intro_complete.
-      all: eauto.
-    + auto.
-  - intros p.
-    destruct p.
-    all: cbn.
-    + apply lookup_complete.
-      auto.
-    + repeat erewrite elim_complete.
-      all: eauto.
-      cbn.
-      auto.
-    + repeat erewrite elim_complete.
-      all: eauto.
-      cbn.
-      auto.
-    + apply intro_complete.
-      auto.
-Qed.
-
-Theorem intro_preserve {ρ v N}:
-    ρ ⊢ v ⇓ N →
-    ∀ {Γ},
-      Jp ρ Γ →
-      ∀ {t},
-      Γ ⊢ v in t → nil ⊢ N in t
-with elim_preserve {ρ V N}:
-    bigV ρ V N →
-    ∀ {Γ},
-      Jp ρ Γ →
-      ∀ {t}, JV Γ V t → nil ⊢ N in t
-.
-Proof using.
-  - intros p.
-    destruct p.
-    all: intros ? ? ? q.
-    all: inversion q.
-    all: subst.
-    all: cbn.
-    + constructor.
-    + constructor.
-      all: eauto.
-    + eapply elim_preserve.
-      all: eauto.
-  - intros p.
-    destruct p.
-    all: intros ? ? ? q.
-    all: inversion q.
-    all: subst.
-    all: cbn.
-    + induction H0.
-      1: inversion H3.
-      inversion H3.
-      all: subst.
-      all: inversion H.
-      all: subst.
-      all: try contradiction.
-      * auto.
-      * eapply IHJp.
-        all: eauto.
-        constructor.
-        auto.
-    + assert (H2' := elim_preserve _ _ _ p _ H _ H2).
-      cbn in H2'.
-      inversion H2'.
-      subst.
-      auto.
-    + assert (H2' := elim_preserve _ _ _ p _ H _ H2).
-      cbn in H2'.
-      inversion H2'.
-      subst.
-      auto.
-    + eapply intro_preserve.
-      all: eauto.
-Qed.
-
-Theorem big_unique {ρ V N N'}:
-    bigV ρ V N → bigV ρ V N' → N = N'.
-Proof using.
-  intros p q.
-  assert (p' := elim_complete p).
-  assert (q' := elim_complete q).
-  rewrite p' in q'.
-  inversion q'.
-  auto.
-Qed.
-
-Theorem intro_normal {ρ v Γ t}:
-    Jp ρ Γ →
-   Γ ⊢ v in t →
-   ∃ N, ρ ⊢ v ⇓ N
-with elim_normal {ρ V Γ t}:
-    Jp ρ Γ →
-   JV Γ V t →
-   ∃ N, bigV ρ V N.
-Proof using.
-  - intros q p.
-    destruct v.
-    all: inversion p.
-    all: subst.
-    + exists N_tt.
-      constructor.
-    + destruct (intro_normal _ _ _ _ q H2) as [N1 s1].
-      destruct (intro_normal _ _ _ _ q H4) as [N2 s2].
-      exists (N_fanout N1 N2).
-      constructor.
-      all: auto.
-    + destruct (elim_normal _ _ _ _ q H1) as [N s].
-      exists N.
-      constructor.
-      auto.
-  - intros q p.
-    destruct V.
-    all: inversion p.
-    all: subst.
-    + clear p.
-      induction q.
-      1: inversion H1.
-      inversion H1.
-      all: subst.
-      * exists N.
-        constructor.
-        constructor.
-      * destruct (IHq H7) as [N' ?].
-        exists N'.
-        constructor.
-        inversion H0.
-        subst.
-        constructor.
-        all: eauto.
-    + destruct (elim_normal _ _ _ _ q H1) as [N s].
-      assert (wf := elim_preserve s q H1).
-      destruct N.
-      all: inversion wf.
-      subst.
-      exists N1.
-      econstructor.
-      eauto.
-    + destruct (elim_normal _ _ _ _ q H1) as [N s].
-      assert (wf := elim_preserve s q H1).
-      destruct N.
-      all: inversion wf.
-      subst.
-      exists N2.
-      econstructor.
-      eauto.
-    + destruct (intro_normal _ _ _ _ q H3) as [N s].
-      exists N.
-      constructor.
-      auto.
-Qed.
-
-Lemma big_normal {ρ N}: ρ ⊢ N ⇓ N.
-Proof using.
-  induction N.
-  all: cbn.
-  all: constructor.
-  all: auto.
-Qed.
-
-Lemma subst_var {x v}:
-  subst_term (V_var x) x v = v
-with
-  subst_var_elim {x V}:
-  subst_expr (V_var x) x V = V.
-Proof.
-  - destruct v.
-    all: cbn.
-    all: auto.
-    + repeat rewrite subst_var.
-      auto.
-    + rewrite subst_var_elim.
-      auto.
-  - destruct V.
-    all: cbn.
-    all: auto.
-    + destruct (eq_var x0 x).
-      all: auto.
-    + rewrite subst_var_elim.
-      auto.
-    + rewrite subst_var_elim.
-      auto.
-    + rewrite subst_var.
-      auto.
-Qed.
-
-Lemma subst_normal {V x N}: subst_term V x N = N.
-Proof using.
-  induction N.
-  1: reflexivity.
-  cbn.
-  rewrite IHN1, IHN2.
-  reflexivity.
-Qed.
-
-Lemma
-  subst_preserve:
-  ∀ {Γ V' t x},
-    JV Γ V' t →
-  ∀ {v t'},
-    cons (x, t) Γ ⊢ v in t' →
-    Γ ⊢ subst_term V' x v in t'
-with
-  subst_preserve_elim:
-  ∀ {Γ V' t x},
-    JV Γ V' t →
-  ∀ {V t'},
-    JV (cons (x, t) Γ) V t' →
-    JV Γ (subst_expr V' x V) t'
-.
-Proof using.
-  - intros Γ V' t x p v.
-    destruct v.
-    all: cbn.
-    all: intros t' q.
-    all: inversion q.
-    all: subst.
-    all: try (econstructor; eauto).
-  - intros Γ V' t x p V.
-    destruct V.
-    all: cbn.
-    all: intros t' q.
-    all: inversion q.
-    all: subst.
-    all: try (econstructor; eauto).
-    destruct eq_var.
-    + subst.
-      inversion H1.
-      2: contradiction.
-      subst.
-      auto.
-    + inversion H1.
-      1: contradiction.
-      subst.
-      constructor.
-      auto.
-Qed.
-
-Lemma
-  subst_expr_assoc {x f g h}:
-  subst_expr f x (subst_expr g x h) = subst_expr (subst_expr f x g) x h
-with
-  subst_term_assoc {x f g h}:
-  subst_term f x (subst_term g x h) = subst_term (subst_expr f x g) x h
-.
-Proof using.
-  - destruct h.
-    all: cbn.
-    + destruct eq_var.
-      1: auto.
-      cbn.
-      destruct eq_var.
-      1: subst; contradiction.
-      auto.
-    + rewrite subst_expr_assoc.
-      auto.
-    + rewrite subst_expr_assoc.
-      auto.
-    + rewrite subst_term_assoc.
-      auto.
-  - destruct h.
-    all: cbn.
-    + auto.
-    + repeat rewrite subst_term_assoc.
-      auto.
-    + rewrite subst_expr_assoc.
-      auto.
-Qed.
-
-Lemma map_term {Γ Γ'}:
-  (∀ x t, mem x t Γ → mem x t Γ') →
-  ∀ {v t}, Γ ⊢ v in t → Γ' ⊢ v in t
-with map_expr {Γ Γ'}:
-  (∀ x t, mem x t Γ → mem x t Γ') →
-  ∀ {V t}, JV Γ V t → JV Γ' V t.
-Proof.
-  - intros f ? ? p.
-    destruct v.
-    all: inversion p.
-    all: subst.
-    all: clear p.
-    + constructor.
-    + constructor.
-      * eauto.
-      * eauto.
-    + constructor.
-      eauto.
-  - intros f ? ? p.
-    destruct V.
-    all: inversion p.
-    all: subst.
-    all: clear p.
-    + constructor.
-      auto.
-    + econstructor.
-      eauto.
-    + econstructor.
-      eauto.
-    + econstructor.
-      eauto.
-Qed.
-
-Definition oftype Γ t := { V | JV Γ V t }.
-
-Definition equiv {Γ t} (p q: oftype Γ t): Prop :=
-  ∀ ρ, Jp ρ Γ →
-  ∃ N, bigV ρ (proj1_sig p) N ∧ bigV ρ (proj1_sig q) N.
+Definition equiv {Γ t} (p q: oftype Γ t): Prop := proj1_sig p = proj1_sig q.
 
 Instance equiv_Reflexive Γ t: Reflexive (@equiv Γ t).
 Proof.
   unfold Reflexive.
-  intros V ρ q.
-  destruct (elim_normal q (proj2_sig V)) as [N ?].
-  exists N.
-  split.
-  all: auto.
+  reflexivity.
 Qed.
 
 Instance equiv_Transitive Γ t: Transitive (@equiv Γ t).
 Proof.
-  unfold Transitive.
-  intros ? ? ? f g ? q.
-  destruct (f _ q) as [f' [? fq]], (g _ q) as [g' [gq ?]].
-  assert (eqv := big_unique fq gq).
-  subst.
-  exists g'.
-  split.
-  all: auto.
+  unfold Transitive, equiv.
+  intros ? ? ? f g.
+  rewrite f, g.
+  auto.
 Qed.
 
 Instance equiv_Symmetric Γ t: Symmetric (@equiv Γ t).
 Proof.
-  unfold Symmetric.
-  intros ? ? f ? q.
-  destruct (f _ q) as [f' [? ?]].
-  exists f'.
-  split.
-  all: auto.
+  unfold Symmetric, equiv.
+  intros ? ? f.
+  auto.
 Qed.
 
 Instance equiv_Equivalence Γ t: Equivalence (@equiv Γ t) := {
@@ -603,3 +499,24 @@ Instance equiv_Equivalence Γ t: Equivalence (@equiv Γ t) := {
 Instance oftype_Setoid Γ t: Setoid (oftype Γ t) := {
     equiv := @equiv Γ t ;
 }.
+
+Instance subrelation_equiv_eq {Γ t}: subrelation (@equiv Γ t) (@eq _).
+Proof.
+  intros v v'.
+  destruct v as [? p], v' as [? p'].
+  cbn.
+  unfold equiv.
+  cbn.
+  intros r.
+  subst.
+  replace p with p'.
+  1: auto.
+  generalize dependent p.
+  generalize dependent p'.
+  destruct typecheck.
+  2: contradiction.
+  cbn.
+  intros.
+  destruct p', p.
+  auto.
+Qed.
